moving specs towards combinators and adding missing functions to endianness

code/lib/FStar.Endianness.fst
@@ -5,66 +5,76 @@ open FStar.Ghost
 open FStar.Mul
 open FStar.Int.Cast
 
+module U8 = FStar.UInt8
 
-// should move to Int.Cast!
-#set-options "--z3rlimit 30"
-let uint128_to_uint8 (a:UInt128.t) : Tot (b:UInt8.t{UInt8.v b = UInt128.v a % pow2 8}) = 
-  Math.Lemmas.pow2_modulo_modulo_lemma_2 (UInt128.v a) 64 8;
-  uint64_to_uint8 (uint128_to_uint64 a)
+let u8  = UInt8.t
+let u32 = UInt32.t
+let u64 = UInt64.t
 
-// TODO: Add to FStar.Int.Cast, with Kremlin and OCaml support
-val uint8_to_uint128: a:UInt8.t -> Tot (b:UInt128.t{UInt128.v b == UInt8.v a})
-let uint8_to_uint128 a = uint64_to_uint128 (uint8_to_uint64 a)
+#set-options "--initial_fuel 0 --max_fuel 0"
 
-// relocate too?
-val lemma_euclidean_division: r:nat -> b:nat -> q:pos -> Lemma
-  (requires (r < q))
-  (ensures  (r + q * b < q * (b+1)))
-let lemma_euclidean_division r b q = ()
-#reset-options 
+type bytes  = Seq.seq U8.t // Pure sequence of bytes
+
+type  lbytes  (l:nat) = b:bytes   {Seq.length b == l}
+
+(* type lbuffer (l:nat) = b:buffer {Buffer.length b == l} *)
+
+#reset-options
+
+let uint128_to_uint8 (a:UInt128.t) : Tot (b:UInt8.t{UInt8.v b = UInt128.v a % pow2 8})
+  = Math.Lemmas.pow2_modulo_modulo_lemma_2 (UInt128.v a) 64 8;
+    uint64_to_uint8 (uint128_to_uint64 a)
+
+#reset-options "--z3rlimit 20 --initial_fuel 0 --max_fuel 0"
 
 
-// we specify bytestrings as sequences of bytes
 open FStar.Seq
-type bytes  = seq UInt8.t 
-type  lbytes (l:nat) = b:bytes {length b == l}
 
 (* Little endian integer value of a sequence of bytes *)
-let rec little_endian (b:bytes) : Tot (n:nat) (decreases (length b)) =
-  if length b = 0 then 0
+let rec little_endian (b:bytes) : Tot (n:nat) (decreases (Seq.length b)) =
+  if Seq.length b = 0 then 0
   else
     UInt8.v (head b) + pow2 8 * little_endian (tail b)
 
 (* Big endian integer value of a sequence of bytes *)
-let rec big_endian (b:bytes) : Tot (n:nat) (decreases (length b)) = 
-  if length b = 0 then 0 
+let rec big_endian (b:bytes) : Tot (n:nat) (decreases (Seq.length b)) = 
+  if Seq.length b = 0 then 0 
   else
-    UInt8.v (last b) + pow2 8 * big_endian (slice b 0 (length b - 1))
+    UInt8.v (last b) + pow2 8 * big_endian (Seq.slice b 0 (Seq.length b - 1))
 
 #reset-options "--initial_fuel 1 --max_fuel 1"
 
-val little_endian_null: len:nat{len < 16} -> Lemma (little_endian (create len 0uy) == 0)
+val little_endian_null: len:nat{len < 16} -> Lemma
+  (little_endian (Seq.create len 0uy) == 0)
 let rec little_endian_null len =
-  if len <> 0 then
+  if len = 0 then ()
+  else
     begin
-      lemma_eq_intro (slice (create len 0uy) 1 len) (create (len - 1) 0uy);
-      assert (little_endian (create len 0uy) == 0 + pow2 8 * little_endian (slice (create len 0uy) 1 len));
-      little_endian_null (len - 1)
+    Seq.lemma_eq_intro (Seq.slice (Seq.create len 0uy) 1 len)
+		       (Seq.create (len - 1) 0uy);
+    assert (little_endian (Seq.create len 0uy) ==
+      0 + pow2 8 * little_endian (Seq.slice (Seq.create len 0uy) 1 len));
+    little_endian_null (len - 1)
     end
 
-val little_endian_singleton: n:UInt8.t -> Lemma (little_endian (create 1 n) == UInt8.v n)
+val little_endian_singleton: n:UInt8.t -> Lemma
+  (little_endian (Seq.create 1 n) == UInt8.v n)
 let little_endian_singleton n =
-  assert (little_endian (create 1 n) ==
-    UInt8.v (index (create 1 n) 0) + pow2 8 *
-    little_endian (slice (create 1 n) 1 1))
+  assert (little_endian (Seq.create 1 n) ==
+    UInt8.v (Seq.index (Seq.create 1 n) 0) + pow2 8 *
+    little_endian (Seq.slice (Seq.create 1 n) 1 1))
+
 
 #reset-options "--initial_fuel 1 --max_fuel 1 --z3rlimit 50"
 
 val little_endian_append: w1:bytes -> w2:bytes -> Lemma
+  (requires True)
   (ensures
-    little_endian (w1 @| w2) == little_endian w1 + pow2 (8 * length w1) * little_endian w2)
-  (decreases (length w1))
+    little_endian (Seq.append w1 w2) ==
+    little_endian w1 + pow2 (8 * Seq.length w1) * little_endian w2)
+  (decreases (Seq.length w1))
 let rec little_endian_append w1 w2 =
+  let open FStar.Seq in
   if length w1 = 0 then
     begin
     assert_norm (pow2 (8 * 0) == 1);
@@ -94,47 +104,58 @@ let rec little_endian_append w1 w2 =
     assert (UInt8.v (index w1 0) + pow2 8 * little_endian w1' == little_endian w1)
     end
 
+
+#reset-options "--initial_fuel 1 --max_fuel 1 --z3rlimit 50"
+
+val lemma_euclidean_division: r:nat -> b:nat -> q:pos -> Lemma
+  (requires (r < q))
+  (ensures  (r + q * b < q * (b+1)))
+let lemma_euclidean_division r b q = ()
+
 private val lemma_factorise: a:nat -> b:nat -> Lemma (a + a * b == a * (b + 1))
 let lemma_factorise a b = ()
 
 val lemma_little_endian_is_bounded: b:bytes -> Lemma
-  (ensures little_endian b < pow2 (8 * length b))
+  (requires True)
+  (ensures  (little_endian b < pow2 (8 * Seq.length b)))
   (decreases (Seq.length b))
 let rec lemma_little_endian_is_bounded b =
-  if Seq.length b <> 0 then
+  if Seq.length b = 0 then ()
+  else
     begin
-      let s = slice b 1 (length b) in
-      assert(length s = length b - 1);
-      lemma_little_endian_is_bounded s;
-      assert(UInt8.v (index b 0) < pow2 8);
-      assert(little_endian s < pow2 (8 * length s));
-      assert(little_endian b < pow2 8 + pow2 8 * pow2 (8 * (length b - 1)));
-      lemma_euclidean_division (UInt8.v (index b 0)) (little_endian s) (pow2 8);
-      assert(little_endian b <= pow2 8 * (little_endian s + 1));
-      assert(little_endian b <= pow2 8 * pow2 (8 * (length b - 1)));
-      Math.Lemmas.pow2_plus 8 (8 * (length b - 1));
-      lemma_factorise 8 (length b - 1)
+    let s = Seq.slice b 1 (Seq.length b) in
+    assert(Seq.length s = Seq.length b - 1);
+    lemma_little_endian_is_bounded s;
+    assert(UInt8.v (Seq.index b 0) < pow2 8);
+    assert(little_endian s < pow2 (8 * Seq.length s));
+    assert(little_endian b < pow2 8 + pow2 8 * pow2 (8 * (Seq.length b - 1)));
+    lemma_euclidean_division (UInt8.v (Seq.index b 0)) (little_endian s) (pow2 8);
+    assert(little_endian b <= pow2 8 * (little_endian s + 1));
+    assert(little_endian b <= pow2 8 * pow2 (8 * (Seq.length b - 1)));
+    Math.Lemmas.pow2_plus 8 (8 * (Seq.length b - 1));
+    lemma_factorise 8 (Seq.length b - 1)
     end
 
 val lemma_big_endian_is_bounded: b:bytes -> Lemma
   (requires True)
-  (ensures big_endian b < pow2 (8 * length b))
+  (ensures  (big_endian b < pow2 (8 * Seq.length b)))
   (decreases (Seq.length b))
   [SMTPat (big_endian b)]
 let rec lemma_big_endian_is_bounded b =
-  if Seq.length b <> 0 then
+  if Seq.length b = 0 then ()
+  else
     begin
-      let s = slice b 0 (length b - 1) in
-      assert(length s = length b - 1);
-      lemma_big_endian_is_bounded s;
-      assert(UInt8.v (last b) < pow2 8);
-      assert(big_endian s < pow2 (8 * length s));
-      assert(big_endian b < pow2 8 + pow2 8 * pow2 (8 * (length b - 1)));
-      lemma_euclidean_division (UInt8.v (last b)) (big_endian s) (pow2 8);
-      assert(big_endian b <= pow2 8 * (big_endian s + 1));
-      assert(big_endian b <= pow2 8 * pow2 (8 * (length b - 1)));
-      Math.Lemmas.pow2_plus 8 (8 * (length b - 1));
-      lemma_factorise 8 (length b - 1)
+    let s = Seq.slice b 0 (Seq.length b - 1) in
+    assert(Seq.length s = Seq.length b - 1);
+    lemma_big_endian_is_bounded s;
+    assert(UInt8.v (Seq.last b) < pow2 8);
+    assert(big_endian s < pow2 (8 * Seq.length s));
+    assert(big_endian b < pow2 8 + pow2 8 * pow2 (8 * (Seq.length b - 1)));
+    lemma_euclidean_division (UInt8.v (Seq.last b)) (big_endian s) (pow2 8);
+    assert(big_endian b <= pow2 8 * (big_endian s + 1));
+    assert(big_endian b <= pow2 8 * pow2 (8 * (Seq.length b - 1)));
+    Math.Lemmas.pow2_plus 8 (8 * (Seq.length b - 1));
+    lemma_factorise 8 (Seq.length b - 1)
     end
 
 
@@ -142,14 +163,19 @@ let rec lemma_big_endian_is_bounded b =
 
 val lemma_little_endian_lt_2_128: b:bytes {Seq.length b <= 16} -> Lemma
   (requires True)
-  (ensures little_endian b < pow2 128)
+  (ensures  (little_endian b < pow2 128))
   [SMTPat (little_endian b)]
 let lemma_little_endian_lt_2_128 b =
   lemma_little_endian_is_bounded b;
   if Seq.length b = 16 then ()
   else Math.Lemmas.pow2_lt_compat 128 (8 * Seq.length b)
 
-#reset-options "--z3rlimit 30 --max_fuel 1 --initial_fuel 1"
+
+#reset-options "--z3rlimit 100 --max_fuel 1 --initial_fuel 1"
+
+val uint8_to_uint128: a:UInt8.t -> Tot (b:UInt128.t{UInt128.v b == UInt8.v a})
+let uint8_to_uint128 a = uint64_to_uint128 (uint8_to_uint64 a)
+
 
 // turns an integer into a bytestream, little-endian
 val little_bytes: 
@@ -157,7 +183,7 @@ val little_bytes:
   Tot (b:lbytes (v len) {n == little_endian b}) (decreases (v len))
 let rec little_bytes len n = 
   if len = 0ul then 
-    createEmpty 
+    Seq.createEmpty 
   else
     let len = len -^ 1ul in 
     let byte = UInt8.uint_to_t (n % 256) in
@@ -171,9 +197,10 @@ let rec little_bytes len n =
 
 #reset-options "--initial_fuel 1 --max_fuel 1 --initial_ifuel 0 --max_ifuel 0"
 
+
 (* injectivity proofs for byte encodings *) 
 
-type word = b:seq UInt8.t {length b <= 16}
+type word = b:Seq.seq UInt8.t {Seq.length b <= 16}
 open FStar.Math.Lib
 open FStar.Math.Lemmas
 
@@ -183,7 +210,7 @@ private let endian_is_injective q r q' r' : Lemma
   lemma_mod_injective (pow2 8) (UInt8.v r) (UInt8.v r')
 
 private let big_endian_step (b:word{length b > 0}) : 
-  Lemma (big_endian b = UInt8.v (last b) + pow2 8 * big_endian (slice b 0 (length b - 1))) =
+  Lemma (big_endian b = U8.v (last b) + pow2 8 * big_endian (slice b 0 (length b - 1))) =
   ()
 
 #reset-options "--z3rlimit 100"
@@ -233,14 +260,14 @@ let lemma_little_endian_is_injective_2 b len =
 private val lemma_little_endian_is_injective_3: b:word -> b':word -> len:pos{len <= length b /\ len <= length b'} -> Lemma
   (requires 
     slice b (length b - (len - 1)) (length b) == slice b' (length b' - (len-1)) (length b') /\ 
-    index b (length b - len) = index b' (length b' - len))
+    Seq.index b (length b - len) = Seq.index b' (length b' - len))
   (ensures slice b (length b - len) (length b) == slice b' (length b' - len) (length b'))
 let lemma_little_endian_is_injective_3 b b' len =
   lemma_eq_intro (slice b (length b - len) (length b)) (cons (index b (length b - len)) (slice b (length b - (len-1)) (length b)));
   lemma_eq_intro (slice b' (length b' - len) (length b')) (cons (index b' (length b' - len)) (slice b' (length b' - (len-1)) (length b')))
 
 private let little_endian_step (b:word{length b > 0}): 
-  Lemma (little_endian b = UInt8.v (head b) + pow2 8 * little_endian (tail b)) 
+  Lemma (little_endian b = U8.v (head b) + pow2 8 * little_endian (tail b)) 
   = ()
 
 val lemma_little_endian_is_injective: b:word -> b':word -> len:nat{len <= length b /\ len <= length b'} -> Lemma
@@ -265,6 +292,70 @@ val lemma_little_endian_inj: b:word -> b':word {length b = length b'} -> Lemma
   (ensures b == b')
 let lemma_little_endian_inj b b' =
   let len = length b in 
-  lemma_eq_intro b (slice b 0  len);
-  lemma_eq_intro b' (slice b' 0  len);
+  Seq.lemma_eq_intro b (Seq.slice b 0  len);
+  Seq.lemma_eq_intro b' (Seq.slice b' 0  len);
   lemma_little_endian_is_injective b b' len
+
+
+val uint32_bytes: 
+  len:UInt32.t {v len <= 4} -> n:UInt32.t {UInt32.v n < pow2 (8 * v len)} -> 
+  Tot (b:lbytes (v len) { UInt32.v n == little_endian b}) (decreases (v len))
+let rec uint32_bytes len n = 
+  if len = 0ul then 
+    let e = Seq.createEmpty #UInt8.t in
+    assert_norm(0 = little_endian e);
+    e
+  else
+    let len = len -^ 1ul in 
+    let byte = uint32_to_uint8 n in
+    let n1 = n in (* n defined in FStar.UInt32, so was shadowed, so renamed into n1 *)
+    let n' = FStar.UInt32.(n1 >>^ 8ul) in 
+    assert(v n = UInt8.v byte + 256 * v n');
+    Math.Lemmas.pow2_plus 8 (8 * v len);
+    assert_norm (pow2 8 == 256);
+    assert(v n' < pow2 (8 * v len ));
+    let b' = uint32_bytes len n'
+    in 
+    Seq.cons byte b'
+
+val uint32_be: 
+  len:UInt32.t {v len <= 4} -> n:UInt32.t {UInt32.v n < pow2 (8 * v len)} -> 
+  Tot (b:lbytes (v len) { UInt32.v n == big_endian b}) (decreases (v len))
+let rec uint32_be len n = 
+  if len = 0ul then 
+    let e = Seq.createEmpty #UInt8.t in
+    assert_norm(0 = big_endian e);
+    e
+  else
+    let len = len -^ 1ul in 
+    let byte = uint32_to_uint8 n in
+    let n1 = n in (* n shadowed by FStar.UInt32.n *)
+    let n' = FStar.UInt32.(n1 >>^ 8ul) in 
+    assert(v n = UInt8.v byte + 256 * v n');
+    Math.Lemmas.pow2_plus 8 (8 * v len);
+    assert_norm (pow2 8 == 256);
+    assert(v n' < pow2 (8 * v len ));
+    let b' = uint32_be len n'
+    in 
+    Seq.snoc b' byte 
+
+#reset-options "--z3rlimit 400"
+
+// turns an integer into a bytestream, big-endian
+val big_bytes: 
+  len:UInt32.t -> n:nat{n < pow2 (8 * v len)} ->
+  Tot (b:lbytes (v len) {n == big_endian b}) (decreases (v len))
+let rec big_bytes len n = 
+  if len = 0ul then 
+    Seq.createEmpty 
+  else
+    let len = len -^ 1ul in 
+    let byte = UInt8.uint_to_t (n % 256) in
+    let n' = n / 256 in 
+    Math.Lemmas.pow2_plus 8 (8 * v len);
+    assert(n' < pow2 (8 * v len ));
+    let b' = big_bytes len n' in
+    let b'' = Seq.create 1 byte in
+    let b = Seq.append b' b'' in
+    assert(Seq.equal b' (Seq.slice b 0 (v len)));
+    b
