specs/Spec.Chacha20.fst
@@ -10,10 +10,6 @@ open Spec.Lib
 
 #set-options "--initial_fuel 0 --max_fuel 0 --z3rlimit 100"
 
-// left rotation by s bits; could go elsewhere
-let op_Less_Less_Less (a:UInt32.t) (s:UInt32.t {v s<32}) : Tot UInt32.t =
-  (a <<^ s) |^ (a >>^ (32ul -^ s))
-
 let keylen = 32 (* in bytes *)
 let blocklen = 64  (* in bytes *)
 let noncelen = 12 (* in bytes *)
@@ -59,21 +55,23 @@ let double_round: shuffle =
 let rec rounds : shuffle = 
     iter 10 double_round (* 20 rounds *)
 
-let chacha20_core (s:state) = 
+let chacha20_core (s:state) : Tot state = 
     let s' = rounds s in
     map2 (fun x y -> x +%^ y) s s'
 
 (* state initialization *) 
 
-let constants = [0x61707865ul; 0x3320646eul; 0x79622d32ul; 0x6b206574ul]
+unfold let constants = [0x61707865ul; 0x3320646eul; 0x79622d32ul; 0x6b206574ul]
 
-let setup (k:key) (n:nonce) (c:counter): state =
+// JK: I have to add those assertions to typechecks, would be nice to get rid of it
+let setup (k:key) (n:nonce) (c:counter): Tot state =
+  assert_norm(List.Tot.length constants = 4); assert_norm(List.Tot.length [UInt32.uint_to_t c] = 1);
   createL constants @|
   uint32s_from_le 8 k @|
   createL [UInt32.uint_to_t c] @| 
   uint32s_from_le 3 n
 
-let chacha20_block (k:key) (n:nonce) (c:counter): block =
+let chacha20_block (k:key) (n:nonce) (c:counter): Tot block =
     let st = setup k n c in
     let st' = chacha20_core st in
     uint32s_to_le 16 st'
@@ -94,8 +92,8 @@ let chacha20_encrypt_bytes key nonce counter m =
     Spec.CTR.counter_mode chacha20_ctx chacha20_cipher key nonce counter m
 
 
-unfold let test_plaintext : lbytes 114 = createL [
-    0x4cuy; 0x61uy; 0x64uy; 0x69uy; 0x65uy; 0x73uy; 0x20uy; 0x61uy; 
+unfold let test_plaintext = [
+    0x4cuy; 0x61uy; 0x64uy; 0x69uy; 0x65uy; 0x73uy; 0x20uy; 0x61uy;
     0x6euy; 0x64uy; 0x20uy; 0x47uy; 0x65uy; 0x6euy; 0x74uy; 0x6cuy;
     0x65uy; 0x6duy; 0x65uy; 0x6euy; 0x20uy; 0x6fuy; 0x66uy; 0x20uy;
     0x74uy; 0x68uy; 0x65uy; 0x20uy; 0x63uy; 0x6cuy; 0x61uy; 0x73uy;
@@ -103,7 +101,7 @@ unfold let test_plaintext : lbytes 114 = createL [
     0x3auy; 0x20uy; 0x49uy; 0x66uy; 0x20uy; 0x49uy; 0x20uy; 0x63uy;
     0x6fuy; 0x75uy; 0x6cuy; 0x64uy; 0x20uy; 0x6fuy; 0x66uy; 0x66uy;
     0x65uy; 0x72uy; 0x20uy; 0x79uy; 0x6fuy; 0x75uy; 0x20uy; 0x6fuy;
-    0x6euy; 0x6cuy; 0x79uy; 0x20uy; 0x6fuy; 0x6euy; 0x65uy; 0x20uy; 
+    0x6euy; 0x6cuy; 0x79uy; 0x20uy; 0x6fuy; 0x6euy; 0x65uy; 0x20uy;
     0x74uy; 0x69uy; 0x70uy; 0x20uy; 0x66uy; 0x6fuy; 0x72uy; 0x20uy;
     0x74uy; 0x68uy; 0x65uy; 0x20uy; 0x66uy; 0x75uy; 0x74uy; 0x75uy;
     0x72uy; 0x65uy; 0x2cuy; 0x20uy; 0x73uy; 0x75uy; 0x6euy; 0x73uy;
@@ -112,7 +110,7 @@ unfold let test_plaintext : lbytes 114 = createL [
     0x74uy; 0x2euy
 ]
 
-unfold let test_ciphertext  = createL [
+unfold let test_ciphertext = [
     0x6euy; 0x2euy; 0x35uy; 0x9auy; 0x25uy; 0x68uy; 0xf9uy; 0x80uy;
     0x41uy; 0xbauy; 0x07uy; 0x28uy; 0xdduy; 0x0duy; 0x69uy; 0x81uy;
     0xe9uy; 0x7euy; 0x7auy; 0xecuy; 0x1duy; 0x43uy; 0x60uy; 0xc2uy;
@@ -130,18 +128,26 @@ unfold let test_ciphertext  = createL [
     0x87uy; 0x4duy
 ]
 
-unfold let test_key:key = createL [
+unfold let test_key = [
     0uy;   1uy;  2uy;  3uy;  4uy;  5uy;  6uy;  7uy;
     8uy;   9uy; 10uy; 11uy; 12uy; 13uy; 14uy; 15uy;
     16uy; 17uy; 18uy; 19uy; 20uy; 21uy; 22uy; 23uy;
     24uy; 25uy; 26uy; 27uy; 28uy; 29uy; 30uy; 31uy
-    ] 
-unfold let test_nonce:nonce = createL [ 
+    ]
+unfold let test_nonce = [
     0uy; 0uy; 0uy; 0uy; 0uy; 0uy; 0uy; 0x4auy; 0uy; 0uy; 0uy; 0uy
-    ] 
+    ]
 
 unfold let test_counter = 1
 
-let test() = 
-    chacha20_encrypt_bytes test_key test_nonce test_counter test_plaintext 
-    = test_ciphertext
+let test() =
+  assert_norm(List.Tot.length test_plaintext = 114);
+  assert_norm(List.Tot.length test_ciphertext = 114);
+  assert_norm(List.Tot.length test_key = 32);
+  assert_norm(List.Tot.length test_nonce = 12);
+  let test_plaintext = createL test_plaintext in
+  let test_ciphertext = createL test_ciphertext in
+  let test_key = createL test_key in
+  let test_nonce = createL test_nonce in
+  chacha20_encrypt_bytes test_key test_nonce test_counter test_plaintext
+  = test_ciphertext
