specs/generic/Spec.Lib.fst
@@ -6,6 +6,7 @@ open FStar.UInt32
 open FStar.Endianness
 
 
+#set-options "--initial_fuel 0 --initial_ifuel 0 --max_fuel 0 --max_ifuel 0"
 
 let rotate_left (a:UInt32.t) (s:UInt32.t {v s<32}) : Tot UInt32.t =
   ((a <<^ s) |^ (a >>^ (32ul -^ s)))
@@ -20,33 +21,38 @@ let byte = UInt8.t
 let bytes = seq UInt8.t
 let lbytes (l:nat) = b:seq UInt8.t {length b = l}
 let op_At f g = fun x -> g (f x)
-let set i x s = upd s i x
+inline_for_extraction
+let set (i:nat) (x:'a) (s:seq 'a{length s > i}) : Tot (seq 'a) = upd s i x
 
-val iter: n:nat -> (f: 'a -> Tot 'a) -> 'a -> 'a
-let rec iter n f x = if n = 0 then x else iter (n-1) f (f x)
-val map2: ('a -> 'b -> Tot 'c) ->
-	  a:seq 'a -> b:seq 'b{length b = length a} ->
-    	  Tot (c:seq 'c{length c = length a}) (decreases (length a))
-let rec map2 f s1 s2 =
-  let len = length s1 in
-  if len = 0 then Seq.createEmpty
-  else
-     let h1 = index s1 0 in
-     let h2 = index s2 0 in
-     let t1 = slice s1 1 len in
-     let t2 = slice s2 1 len in
-     let r = map2 f t1 t2 in
-     cons (f h1 h2) r
+inline_for_extraction
+let iter n f x = Combinators.iter_ n f x
 
+inline_for_extraction
+let map2 f s1 s2 = Combinators.seq_map2 f s1 s2
+
+#set-options "--initial_fuel 0 --max_fuel 0"
 
 let uint32_from_le (b:lbytes 4) : UInt32.t =
     let n = little_endian b  in
-    UInt32.uint_to_t (UInt.to_uint_t 32 n)
+    lemma_little_endian_is_bounded b;
+    UInt32.uint_to_t n
 
 let uint32_to_le (a:UInt32.t) : lbytes 4 =
     little_bytes 4ul (v a)
 
 
+let lemma_uint32_from_le_inj (b:lbytes 4) (b':lbytes 4) : Lemma
+  (requires (uint32_from_le b = uint32_from_le b'))
+  (ensures  (b == b'))
+  = lemma_little_endian_inj b b'
+
+
+let lemma_uint32_to_le_inj (b:UInt32.t) (b':UInt32.t) : Lemma
+  (requires (uint32_to_le b == uint32_to_le b'))
+  (ensures  (b = b'))
+  = ()
+
+// JK: those two should go somewhere else
 val uint32s_from_le: len:nat -> b:lbytes (4 * len) -> Tot (s:seq UInt32.t{length s = len}) (decreases len)
 let rec uint32s_from_le len src =
   if len = 0 then Seq.createEmpty #UInt32.t
@@ -64,3 +70,82 @@ let rec uint32s_to_le len src =
     let t = slice src 1 len in
     Seq.append (uint32_to_le h)
                (uint32s_to_le (len-1) t)
+
+
+#reset-options "--initial_fuel 1 --max_fuel 1 --z3rlimit 20"
+
+private let lemma_uint32s_from_le_def_0 (len:nat{len = 0}) (b:lbytes (4*len)) : Lemma
+  (uint32s_from_le len b == Seq.createEmpty)
+  = ()
+private let lemma_uint32s_from_le_def_1 (len:nat{len > 0}) (b:lbytes (4*len)) : Lemma
+  (uint32s_from_le len b == Seq.cons (uint32_from_le (slice b 0 4))
+                                     (uint32s_from_le (len-1) (slice b 4 (4*len))))
+  = ()
+
+
+private let lemma_uint32s_to_le_def_0 (len:nat{len = 0}) (s:seq UInt32.t{length s = len}) : Lemma
+  (uint32s_to_le len s == Seq.createEmpty)
+  = ()
+private let lemma_uint32s_to_le_def_1 (len:nat{len > 0}) (s:seq UInt32.t{length s = len}) : Lemma
+  (uint32s_to_le len s == Seq.append (uint32_to_le (index s 0))
+                                     (uint32s_to_le (len-1) (slice s 1 (len))))
+  = ()
+
+
+#reset-options "--initial_fuel 0 --max_fuel 0 --z3rlimit 20"
+
+let rec lemma_uint32s_from_le_inj (len:nat) (b:lbytes (4 * len)) (b':lbytes (4 * len)) : Lemma
+  (requires (uint32s_from_le len b == uint32s_from_le len b'))
+  (ensures  (b == b'))
+  = if len = 0 then (lemma_uint32s_from_le_def_0 len b; lemma_uint32s_from_le_def_0 len b';
+      Seq.lemma_eq_intro b b')
+    else (let h  = slice b 0 4 in
+          let h' = slice b' 0 4 in
+          let t  = slice b 4 (4*len) in
+          let t' = slice b' 4 (4*len) in
+          lemma_uint32s_from_le_def_1 len b;
+          lemma_uint32s_from_le_def_1 len b';
+          Seq.lemma_eq_intro (uint32s_from_le len b) (uint32s_from_le len b');
+          cut (Seq.index (uint32s_from_le len b) 0 == Seq.index (uint32s_from_le len b') 0); 
+          cut (Seq.index (uint32s_from_le len b) 0 == uint32_from_le h);
+          cut (Seq.index (uint32s_from_le len b') 0 == uint32_from_le h');
+          lemma_uint32_from_le_inj h h';
+          Seq.lemma_eq_intro h h';
+          cut (Seq.slice (uint32s_from_le len b) 1 len == Seq.slice (uint32s_from_le len b') 1 len);
+          Seq.lemma_eq_intro (Seq.slice (uint32s_from_le len b) 1 len) (uint32s_from_le (len-1) t);
+          Seq.lemma_eq_intro (Seq.slice (uint32s_from_le len b') 1 len) (uint32s_from_le (len-1) t');
+          lemma_uint32s_from_le_inj (len-1) t t';
+          Seq.lemma_eq_intro t t';
+          Seq.lemma_eq_intro b (h @| t);
+          Seq.lemma_eq_intro b' (h' @| t')
+          )
+
+
+let rec lemma_uint32s_to_le_inj (len:nat) (b:seq UInt32.t{length b = len})
+                                         (b':seq UInt32.t{length b' = len})  : Lemma
+  (requires (uint32s_to_le len b == uint32s_to_le len b'))
+  (ensures  (b == b'))
+  = if len = 0 then (
+      lemma_uint32s_to_le_def_0 len b;
+      lemma_uint32s_to_le_def_0 len b';
+      Seq.lemma_eq_intro b b'
+    ) else (
+      let h  = index b 0 in
+      let h' = index b' 0 in
+      let t  = slice b 1 (len) in
+      let t' = slice b' 1 (len) in
+      lemma_uint32s_to_le_def_1 len b;
+      lemma_uint32s_to_le_def_1 len b';
+      Seq.lemma_eq_intro (uint32s_to_le len b) (uint32s_to_le len b');
+      cut (Seq.slice (uint32s_to_le len b) 0 4 == Seq.slice (uint32s_to_le len b') 0 4);
+      Seq.lemma_eq_intro (Seq.slice (uint32s_to_le len b) 0 4) (uint32_to_le h);
+      Seq.lemma_eq_intro (Seq.slice (uint32s_to_le len b') 0 4) (uint32_to_le h');
+      lemma_uint32_to_le_inj h h';
+      cut (Seq.slice (uint32s_to_le len b) 4 (4*len) == Seq.slice (uint32s_to_le len b') 4 (4*len));
+      Seq.lemma_eq_intro (Seq.slice (uint32s_to_le len b) 4 (4*len)) (uint32s_to_le (len-1) t);
+      Seq.lemma_eq_intro (Seq.slice (uint32s_to_le len b') 4 (4*len)) (uint32s_to_le (len-1) t');
+      lemma_uint32s_to_le_inj (len-1) t t';
+      Seq.lemma_eq_intro t t';
+      Seq.lemma_eq_intro b (cons h t);
+      Seq.lemma_eq_intro b' (cons h' t')
+    )
